Splinter/Journal/PagedJournal.i.dfy
@@ -107,20 +107,13 @@ module PagedJournal {
       }
     }
 
-    function HonorBoundary(boundaryLSN: LSN) : MsgHistory 
-      requires WF()
-      requires boundaryLSN <= messageSeq.seqEnd
-    {
-      if messageSeq.seqStart <= boundaryLSN then messageSeq.DiscardOld(boundaryLSN) 
-      else messageSeq
-    }
 
     function MessageSeqAfterCrop(boundaryLSN: LSN, depth: nat) : MsgHistory
       requires Valid(boundaryLSN)
       requires CanCropHeadRecords(boundaryLSN, depth+1)
     {
       CanCropMoreYieldsSome(boundaryLSN, depth, depth+1);
-      CropHeadRecords(boundaryLSN, depth).value.HonorBoundary(boundaryLSN)
+      CropHeadRecords(boundaryLSN, depth).value.messageSeq.MaybeDiscardOld(boundaryLSN)
     }
   }
 
@@ -128,7 +121,7 @@ module PagedJournal {
     decreases depth, 1
   {
     if ojr.None?
-    then depth==0
+    then depth == 0
     else ojr.value.CanCropHeadRecords(boundaryLSN, depth)
   }
 
